feat(HOTG) split addition file + cleanup

HOTG/Arithmetics/Arithmetics.thy
@@ -1,411 +1,11 @@
 theory Arithmetics
   imports
-    Functions_Restrict
-    Mem_Trans
-    Union_Intersection
-    Foundation
-    Axioms
-    Transport.HOL_Syntax_Bundles_Groups
-    Transport.HOL_Syntax_Bundles_Orders
-    Replacement_Predicates
+    Set_Add
 begin
-
-unbundle no_HOL_ascii_syntax
-
-lemma "{f x | x \<in> (X \<union> Y)} = {f x | x \<in> X} \<union> {f x | x \<in> Y}"
-  by blast
-
-lemma mem_unionI:
-  assumes "Y \<in> X"  "x \<in> Y"
-  shows "x \<in> \<Union>X" 
-  using assms by auto
 
 paragraph \<open>Summary\<close>
 text \<open>Translation of generalised arithmetics from
 \<^url>\<open>https://www.isa-afp.org/entries/ZFC_in_HOL.html\<close>.\<close>
-
-unbundle no_HOL_ascii_syntax
-unbundle no_HOL_groups_syntax
-unbundle no_HOL_order_syntax
-
-(*TODO Kevin: rename to binary_relation_restrict*)
-unbundle no_restrict_syntax
-
-unbundle no_HOL_groups_syntax
-
-abbreviation "zero_set \<equiv> {}"
-abbreviation "one_set \<equiv> {zero_set}"
-
-bundle hotg_set_zero_syntax begin notation zero_set ("0") end
-bundle no_hotg_set_zero_syntax begin no_notation zero_set ("0") end
-
-bundle hotg_set_one_syntax begin notation one_set ("1") end
-bundle no_hotg_set_one_syntax begin no_notation one_set ("1") end
-
-unbundle
-  hotg_set_zero_syntax
-  hotg_set_one_syntax
-
-
-overloading
-  fun_restrict_set \<equiv> "fun_restrict :: (set \<Rightarrow> 'a) \<Rightarrow> set \<Rightarrow> set \<Rightarrow> 'a"
-begin
-  definition "fun_restrict_set f X x \<equiv> if x \<in> X then f x else undefined"
-end
-
-lemma fun_restrict_set_eq_fun_restrict [simp]: "(f :: set \<Rightarrow> 'a)\<restriction>\<^bsub>X\<^esub> = f\<restriction>\<^bsub>mem_of X\<^esub>"
-  unfolding fun_restrict_set_def by auto
-
-axiomatization transrec :: "((set \<Rightarrow> 'a) \<Rightarrow> set \<Rightarrow> 'a) \<Rightarrow> set \<Rightarrow> 'a"
-  where transrec_eq: "transrec f X = f ((transrec f)\<restriction>\<^bsub>X\<^esub>) X"
-
-definition "image f A \<equiv> {f x | x \<in> A}"
-
-lemma image_eq_repl [simp]: "image f A = {f x | x \<in> A}"
-  unfolding image_def by simp
-
-lemma repl_fun_restrict_mem_eq_repl [simp]: "{f\<restriction>\<^bsub>A\<^esub> x | x \<in> A} = {f x | x \<in> A}"
-  by simp
-
-
-paragraph \<open>Transitive Closure\<close>
-
-definition "mem_trans_closure \<equiv> transrec (\<lambda>f x. x \<union> \<Union>(image f x))"
-
-lemma mem_trans_closure_eq_bin_union_repl:
-  "mem_trans_closure X = X \<union> \<Union>{mem_trans_closure x | x \<in> X}"
-  by (simp add: mem_trans_closure_def transrec_eq[where ?X=X])
-
-lemma subset_mem_trans_closure: "X \<subseteq> mem_trans_closure X"
-  by (auto simp:mem_trans_closure_eq_bin_union_repl[where ?X= X])
-
-corollary mem_mem_trans_closure_if_mem: "X \<in> Y \<Longrightarrow> X \<in> mem_trans_closure Y"
-  using subset_mem_trans_closure by blast
-
-lemma mem_trans_closure_empty_eq_empty [simp]: "mem_trans_closure {} = {}"
-  by (simp add: mem_trans_closure_eq_bin_union_repl[where ?X="{}"])
-
-(*TODO Kevin: rename mem_trans to mem_trans_closed*)
-lemma mem_trans_mem_trans_closure: "mem_trans (mem_trans_closure X)"
-proof (induction X rule: mem_induction)
-  case (mem X)
-  show ?case
-  proof (rule mem_transI')
-    fix x y assume "x \<in> mem_trans_closure X" "y \<in> x"
-    then have "x \<in> X \<union> \<Union>{mem_trans_closure x | x \<in> X}" (is "_ \<in> _ \<union> ?tmem")
-      by (simp flip: mem_trans_closure_eq_bin_union_repl)
-    then consider (memX) "x \<in> X" | (memtmem) "x \<in> ?tmem" by blast
-    then show "y \<in> mem_trans_closure X"
-    proof cases
-      case memX
-      moreover have "y \<in> mem_trans_closure x" using \<open>y \<in> x\<close> subset_mem_trans_closure by blast
-      ultimately show ?thesis by (subst mem_trans_closure_eq_bin_union_repl) blast
-    next
-      case memtmem
-      then obtain z where "x \<in> mem_trans_closure z" "z \<in> X" by auto
-      with \<open>y \<in> x\<close> mem.IH \<open>z \<in> X\<close> show ?thesis by (subst mem_trans_closure_eq_bin_union_repl) blast
-    qed
-  qed
-qed
-
-paragraph \<open>Less-Than Order\<close>
-
-definition "lt X Y \<equiv> X \<in> mem_trans_closure Y"
-
-bundle hotg_lt_syntax begin notation lt (infix "<" 60) end
-bundle no_hotg_lt_syntax begin no_notation lt (infix "<" 60) end
-unbundle hotg_lt_syntax
-
-lemma lt_iff_mem_trans_closure: "X < Y \<longleftrightarrow> X \<in> mem_trans_closure Y"
-  unfolding lt_def by simp
-
-lemma lt_if_lt_if_mem [trans]:
-  assumes "y \<in> Y"
-  and "Y < X"
-  shows "y < X"
-  using assms mem_trans_mem_trans_closure unfolding lt_iff_mem_trans_closure by auto
-
-find_theorems name:"not_mem_if_eq"
-
-lemma not_mem_trans_closure [iff]: "X \<notin> mem_trans_closure X"
-proof
-  assume "X \<in> mem_trans_closure X"
-  hence "X \<in> X \<union> \<Union>{mem_trans_closure x | x \<in> X}" 
-    by (simp add:mem_trans_closure_eq_bin_union_repl[where ?X =X])
-  then consider (self) "X \<in> X" | (union) "X \<in> \<Union>{mem_trans_closure x | x \<in> X}" by blast
-  then show False
-  proof cases
-    case union
-      then show ?thesis
-      proof (induction X rule: mem_induction)
-        case (mem X)
-        then obtain y where "y \<in> X" and "X \<in> mem_trans_closure y" by blast
-        then have "X < y" by (simp add:lt_iff_mem_trans_closure)
-        then have "y < y" using  \<open>y \<in> X\<close> by (auto simp:lt_if_lt_if_mem)
-        then have inTC:"y \<in> mem_trans_closure y" by (simp add: lt_iff_mem_trans_closure)
-        also have uni:"mem_trans_closure y = y \<union> \<Union>{mem_trans_closure yy | yy \<in> y}"
-          by (simp add:mem_trans_closure_eq_bin_union_repl[where ?X =y])
-        also have notself:"y \<notin> y" by auto
-        with uni inTC have "y \<in> \<Union>{mem_trans_closure yy | yy \<in> y}" by auto
-        with mem \<open>y \<in> X\<close> show False by auto
-      qed
-  qed (auto)
-qed
-
-lemma not_lt_self [iff]: "\<not>(X < X)"
-  using lt_iff_mem_trans_closure by auto
-
-
-paragraph\<open>Addition\<close>
-
-definition "add X \<equiv> transrec (\<lambda>addX Y. X \<union> image addX Y)"
-
-bundle hotg_add_syntax begin notation add (infixl "+" 65) end
-bundle no_hotg_add_syntax begin no_notation add (infixl "+" 65) end
-unbundle hotg_add_syntax
-
-lemma add_eq_bin_union_image_add: "X + Y = X \<union> image ((+) X) Y"
-  unfolding add_def by (simp add: transrec_eq)
-
-lemma add_eq_bin_union_repl_add: "X + Y = X \<union> {X + y | y \<in> Y}"
-  unfolding add_def by (simp add: transrec_eq)
-
-lemma mem_addE:
-  assumes "x \<in> (Y + Z)"
-  obtains "x \<in> Y" | z where "z \<in> Z" "x = Y + z"
-  using assms by (auto simp: add_eq_bin_union_image_add[of Y Z])
-
-definition "lift X \<equiv> image ((+) X)"
-
-lemma lift_eq_image_add: "lift X = image ((+) X)"
-  unfolding lift_def by simp
-
-lemma lift_eq_repl_add: "lift X Y = {X + y | y \<in> Y}"
-  using lift_eq_image_add by simp
-
-lemma add_eq_bin_union_lift: "X + Y = X \<union> lift X Y"
-  unfolding lift_eq_image_add by (subst add_eq_bin_union_image_add) simp
-
-lemma lift_bin_union_eq_lift_bin_union_lift: "lift X (A \<union> B) = lift X A \<union> lift X B"
-  by (auto simp: lift_eq_image_add)
-
-lemma lift_union_eq_union_repl_lift: "lift X (\<Union>Y) = \<Union>{lift X y | y \<in> Y}"
-  by (auto simp: lift_eq_image_add)
-
-lemma idx_union_add_eq_add_idx_union:
-  "Y \<noteq> {} \<Longrightarrow> (\<Union>y \<in> Y. X + f y) = X + (\<Union>y \<in> Y. f y)"
-  by (simp add: lift_union_eq_union_repl_lift add_eq_bin_union_lift)
-
-lemma lift_zero_eq_zero [simp]: "lift X {} = {}"
-  by (auto simp: lift_eq_image_add)
-
-lemma add_zero_eq_self [simp]: "X + {} = X"
-  unfolding add_eq_bin_union_lift by simp
-
-lemma lift_one_eq_singleton_self [simp]: "lift X 1 = {X}"
-  unfolding lift_def by simp
-
-definition "succ X \<equiv> X + 1"
-
-lemma succ_eq_add_one: "succ X = X + 1"
-  unfolding succ_def by simp
-
-lemma insert_self_eq_add_one: "insert X X = X + 1"
-  by (auto simp: add_eq_bin_union_lift succ_eq_add_one)
-
-lemma lift_singleton_eq_singleton_add: "lift X {Z} = {X + Z}"
-  unfolding lift_def by simp
-
-lemma lift_singleton_eq_singleton_bin_union_lift: "lift X {Z} = {X \<union> lift X Z}"
-  by (simp only: lift_singleton_eq_singleton_add add_eq_bin_union_lift)
-
-lemma lift_bin_union_singleton_eq_lift_bin_union:
-  "lift X (insert Y Z) = lift X Z \<union> {X \<union> lift X Y}"
-  by (simp flip: lift_singleton_eq_singleton_bin_union_lift lift_bin_union_eq_lift_bin_union_lift)
-
-lemma add_insert_eq_insert_add: "X + insert Y Z = insert (X + Y) (X + Z)"
-  by (auto simp: lift_bin_union_singleton_eq_lift_bin_union add_eq_bin_union_lift)
-
-
-paragraph\<open>Proposition 3.3\<close>
-
-lemma zero_add_eq_self [simp]: "{} + X = X"
-proof (induct X rule: mem_induction)
-  case (mem X)
-  have "{} + X = lift {} X" by (simp add: add_eq_bin_union_lift)
-  also from mem have "... = X" by (simp add: lift_eq_image_add)
-  finally show ?case .
-qed
-
-corollary lift_zero_eq_self [simp]: "lift {} X = X"
-  by (simp add: lift_eq_image_add)
-
-corollary add_eq_zeroE [elim]:
-  assumes "X + Y = 0"
-  obtains "X = 0" "Y = 0"
-  using assms by (auto simp: add_eq_bin_union_lift)
-
-corollary add_eq_zero_iff_and_eq_zero [iff]: "X + Y = 0 \<longleftrightarrow> X = 0 \<and> Y = 0" by auto
-
-lemma add_assoc: "(X + Y) + Z = X + (Y + Z)"
-proof(induct Z rule: mem_induction)
-  case (mem Z)
-  from add_eq_bin_union_lift have "(X + Y) + Z = (X + Y) \<union> (lift (X + Y) Z)" by simp
-  also from lift_eq_repl_add have "... = (X + Y) \<union> {(X + Y) + z | z \<in> Z}" by simp
-  also from add_eq_bin_union_lift have "... = X \<union> (lift X Y) \<union> {(X + Y) + z | z \<in> Z}" by simp
-  also from mem have "... = X \<union> (lift X Y) \<union> {X + (Y + z) | z \<in> Z}" by simp
-  also have "... = X \<union> lift X (Y + Z)"
-  proof-
-    have "lift X (Y + Z) = lift X (Y \<union> lift Y Z)"
-      by (simp add: add_eq_bin_union_lift)
-    also have "... = (lift X Y) \<union> lift X (lift Y Z)"
-      by (simp add: lift_bin_union_eq_lift_bin_union_lift)
-    also have "... = (lift X Y) \<union> {X + (Y + z) | z \<in> Z}"
-      by (simp add: lift_eq_repl_add)
-    finally have "lift X (Y + Z) = (lift X Y) \<union> {X + (Y + z) | z \<in> Z}" .
-    then show ?thesis by auto
-  qed
-    also from add_eq_bin_union_lift have "... = X + (Y + Z)" by simp
-    finally show ?case .
-qed
-
-lemma lift_lift_eq_lift_add: "lift X (lift Y Z) = lift (X + Y) Z"
-  by (simp add: lift_eq_image_add add_assoc)
-
-lemma add_succ_eq_succ_add: "X + succ Y = succ (X + Y)"
-  by (auto simp: succ_eq_add_one add_assoc)
-
-lemma add_mem_add_if_mem:
-  assumes "Y \<in> Z"
-  shows "X + Y \<in> X + Z"
-proof-
-  from assms have "X + Y \<in> {X + z| z \<in> Z}" by auto
-  then show ?thesis by (auto simp: lift_eq_repl_add[of X Z] add_eq_bin_union_lift)
-qed
-
-lemma not_add_lt_left [iff]: "\<not>(X + Y < X)"
-proof
-  assume "X + Y < X"
-  then show "False"
-  proof (induction Y rule: mem_induction)
-    case (mem Y)
-    then show ?case
-    proof (cases "Y = {}")
-      case False
-      then obtain y where sub: "y \<in> Y" by blast
-      with add_mem_add_if_mem mem have sub_in: "X + y \<in> X + Y" by auto
-      with mem have bla: "X + y < X" by (auto intro: lt_if_lt_if_mem)
-      with sub mem.IH show ?thesis by auto
-    qed simp
-  qed
-qed
-
-lemma not_add_mem_left [iff]: "\<not>(X + Y \<in> X)"
-  using subset_mem_trans_closure lt_iff_mem_trans_closure by auto
-
-lemma mem_trans_closure_bin_inter_lift_eq_empty [simp]: "mem_trans_closure X \<inter> lift X Y = {}"
-  by (auto simp: lift_eq_image_add simp flip: lt_iff_mem_trans_closure)
-
-lemma bin_inter_lift_self_eq_empty [simp]: "X \<inter> lift X Y = {}"
-  using mem_trans_closure_bin_inter_lift_eq_empty subset_mem_trans_closure by blast
-
-lemma bin_inter_lift_self_eq_empty_assoc [simp]: "lift X Y \<inter> X = {}"
-  using mem_trans_closure_bin_inter_lift_eq_empty subset_mem_trans_closure by blast
-
-lemma lift_eq_lift_if_bin_union_lift_eq_bin_union_lift:
-  assumes "X \<union> lift X Y = X \<union> lift X Z"
-  shows "lift X Y = lift X Z"
-  using assms bin_inter_lift_self_eq_empty by blast
-
-paragraph\<open>Proposition 3.4\<close>
-
-lemma lift_right_inective:
-  assumes "lift X Y = lift X Z"
-  shows "Y = Z"
-using assms
-proof(induction Y arbitrary: Z rule: mem_induction)
-  case (mem Y)
-  {
-    fix U V u assume uvassms: "U \<in> {Y, Z}" "V \<in> {Y, Z}" "U \<noteq> V" "u \<in> U"
-    with mem have "X + u \<in> lift X V" by (auto simp: lift_eq_repl_add)
-    then obtain v where "v \<in> V" "X + u = X + v" using lift_eq_repl_add by auto
-    then have "X \<union> lift X u  = X \<union> lift X v" by (simp add: add_eq_bin_union_lift)
-    with bin_inter_lift_self_eq_empty have "lift X u = lift X v" by blast
-    with uvassms \<open>v \<in> V\<close> mem.IH have "u \<in> V" by auto
-  }
-  then show ?case by blast
-qed
-
-lemma add_right_inective: "X + Y = X + Z \<Longrightarrow> Y = Z"
-  by (subst (asm) add_eq_bin_union_lift)+
-  (fast dest: lift_eq_lift_if_bin_union_lift_eq_bin_union_lift lift_right_inective)
-
-lemma add_mem_add_iff_mem: "X + Y \<in> X + Z \<longleftrightarrow> Y \<in> Z"
-proof (rule iffI)
-  assume left:"X + Y \<in> X + Z"
-  thus "Y \<in> Z"
-  proof-
-    have "X + Y \<in> X + Z"  by (simp add:left)
-    also have "... = X \<union> lift X Z"
-      by (auto simp: add_eq_bin_union_lift)
-    finally have "X + Y \<in> X \<union> lift X Z" .
-    have not_add_lt_left: "\<not> X + Y \<in> X" by auto
-    with \<open>X + Y \<in> X \<union> lift X Z\<close> have "X + Y \<in> lift X Z" by auto
-    have "lift X Z = {X + z| z \<in> Z}" by (simp add:lift_eq_image_add)
-    then have "X + Y \<in> {X + z| z \<in> Z}" using \<open>X + Y \<in> lift X Z\<close> by simp
-    then obtain z where sub: "z \<in> Z" "X + Y = X + z" by blast
-    then have "Y = z" by (auto simp: add_right_inective)
-    then have "Y \<in> Z" using sub by simp
-    then show ?thesis .
-  qed
-next
-  assume "Y \<in> Z"
-  thus "X + Y \<in> X + Z"
-    by (simp add: add_mem_add_if_mem)
-qed
-
-lemma  sss: "lift X Y \<subseteq> lift X Z \<longleftrightarrow> Y \<subseteq> Z"
-proof(rule iffI)
-  assume left:"lift X Y \<subseteq> lift X Z"
-  then have "{X + y|y \<in> Y} \<subseteq> {X + z|z \<in> Z}" 
-    by (auto simp: lift_eq_repl_add)
-  show "Y \<subseteq> Z" 
-  proof (rule subsetI)
-    fix y assume "y \<in> Y"
-    then have "X + y \<in> {X + z|z \<in> Z}" 
-      using \<open>{X + y|y \<in> Y} \<subseteq> {X + z|z \<in> Z}\<close> by auto
-    then obtain z where "X + y = X + z" and "z \<in> Z" by auto
-    then have "y = z" by (auto simp:add_right_inective)
-    then show "y \<in> Z " using \<open>z \<in> Z\<close> by simp
-  qed
-qed (auto simp: lift_eq_image_add)
-
-corollary add_less_cancel_left [iff]:
-  "X + Y \<subseteq> X + Z \<longleftrightarrow> Y \<subseteq> Z"
-proof(rule iffI)
- assume left:"X + Y \<subseteq> X + Z"
-  thus "Y \<subseteq> Z" 
-  proof-
-    have "X + Y \<subseteq> X + Z"  by (simp add:left)
-    also have "... = X \<union> lift X Z"
-      by (auto simp: add_eq_bin_union_lift)
-    finally have "X + Y \<subseteq> X \<union> lift X Z" .
-    then have sub:"(lift X Y) \<subseteq> X \<union> (lift X Z)" 
-      by (auto simp: add_eq_bin_union_lift)
-    have "lift X Y \<inter> X = {}" by simp
-    with sub have "lift X Y \<subseteq> lift X Z" by blast
-      then show ?thesis by (simp add:sss)
-    qed
-next
-  assume "Y \<subseteq> Z"
-  thus "X + Y \<subseteq> X + Z" 
-  proof-
-    have "lift X Y \<subseteq> lift X Z" using \<open>Y \<subseteq> Z\<close> by (simp add:sss)
-    then show ?thesis 
-      by (auto simp: add_eq_bin_union_lift)
-  qed
-qed
-
 
 
 paragraph\<open>Multiplication\<close>
@@ -419,94 +19,64 @@ unbundle hotg_mul_syntax
 lemma mul_eq_union_repl_lift_mul: "X * Y = \<Union>{lift (X * y) X | y \<in> Y}"
   by (auto simp:mul_def transrec_eq)
 
-lemma elts_multE:
-  assumes "z \<in> (X * Y)"
-  obtains u v where "u \<in> X" "v \<in> Y" "z = X * v + u"
- using mul_eq_union_repl_lift_mul[of X Y] assms lift_eq_image_add by auto
-
-lemma mul_zero_eq_zero: "x * {} = {}"
+lemma mul_zero_eq_zero [simp]: "x * 0 = 0"
   unfolding mul_def by (auto simp: transrec_eq)
 
-lemma mul_one_same: "x * 1 = x"
-  unfolding mul_def by (auto simp: transrec_eq)
+lemma mul_one_eq_self [simp]: "x * 1 = x"
+  by (fastforce simp: mul_eq_union_repl_lift_mul[of _ 1])
 
-lemma mul_set_one_eq_lift: "X * {1} = lift X X"
+lemma mul_singleton_one_eq_lift_self: "X * {1} = lift X X"
 proof-
-  have 1:"\<And>Y.  X * Y = \<Union>{lift (X * y) X | y \<in> Y }"
-    by (simp add:mul_def transrec_eq)
   have "X * {1} = \<Union>{lift (X * y) X | y \<in> {1}}"
-    by (simp add: mul_eq_union_repl_lift_mul[where ?Y="{1}"])
+    by (simp only: mul_eq_union_repl_lift_mul[where ?Y="{1}"])
   also have "... = \<Union>{lift (X * 1) X }" by auto
-  also have "... = \<Union>{lift X X}"
-    by (simp add: mul_one_same)
   also have "... = lift X X" by auto
-  finally have "X * {1} = lift X X" .
-    then show ?thesis by simp
-  qed
-
-lemma mul_two_eq_add: "X * {1, 0} = X + X"
-proof-
-  have "X * {1, 0} = \<Union>{lift (X * y) X | y \<in> {1, 0} }"
-    by (simp add: mul_eq_union_repl_lift_mul[where ?Y="{1,0}"])
-  also have "... = (lift (X*1) X) \<union> (lift (X*{}) X)" by auto
-  also have "... = lift X X \<union> lift {} X" by (simp add: mul_one_same mul_zero_eq_zero)
-  also have "... = X \<union> lift X X" by auto
-  also have "... = X + X" by (simp add: add_eq_bin_union_lift)
   finally show ?thesis .
 qed
 
+lemma mul_two_eq_add: "X * 2 = X + X"
+proof -
+  have "X * 2 = \<Union>{lift (X * y) X | y \<in> 2}"
+    by (simp only: mul_eq_union_repl_lift_mul[where ?Y=2])
+  also have "... = (lift (X * 1) X) \<union> (lift (X * 0) X)" by blast
+  also have "... = X + X" by (auto simp: add_eq_bin_union_lift)
+  finally show ?thesis .
+qed
 
-
-lemma insert_eq_bin_union_set: "insert x y = {x} \<union> y"
-  by simp
-
-lemma mul_insert_eq_bin_union_mul_lift: 
+lemma mul_insert_eq_mul_bin_union_lift_mul:
   "X * (insert Z Y) = (X * Y) \<union> lift (X * Z) X"
   sorry
 
-lemma  mul_mem_add_one_eq_mul_add:
+lemma mul_add_one_eq_mul_add [simp]:
   "X * (Y + 1) = X * Y + X"
 proof -
-  have "insert Y Y = Y + 1"
-    by (simp add: insert_self_eq_add_one[where ?X = Y])
-  also have "X * (insert Y Y) = (X * Y) \<union> lift (X * Y) X"
-    by (simp add: mul_insert_eq_bin_union_mul_lift)
-  then have " X * (insert Y Y) = (X * Y) + X"
-    by (simp add: add_eq_bin_union_lift)
-  then show "X * (Y + 1) = (X * Y) + X"
-    using \<open>insert Y Y = Y + 1\<close> by simp
+  have "X * (Y + 1) = X * (insert Y Y)" by (simp only: insert_self_eq_add_one[where ?X = Y])
+  also have "... = (X * Y) \<union> lift (X * Y) X" by (simp only: mul_insert_eq_mul_bin_union_lift_mul)
+  also have " ... = (X * Y) + X" by (simp add: add_eq_bin_union_lift)
+  finally show ?thesis .
 qed
 
 lemma zero_mul_eq_zero [simp]: "0 * X = 0"
-proof (induction X rule:mem_induction)
-  case (mem X)
-  then show ?case 
-    by (subst mul_eq_union_repl_lift_mul) auto
-qed
+  by (induction X, subst mul_eq_union_repl_lift_mul) auto
 
 lemma one_mul_eq_one [simp]: "1 * X = X"
-proof (induction X rule:mem_induction)
-  case (mem X)
-  then show ?case
-    by (auto simp: mem mul_eq_union_repl_lift_mul[where ?Y = X])
-qed 
+proof (induction X)
+  case (mem x)
+  then show ?case by (auto simp: mul_eq_union_repl_lift_mul[where ?Y = x])
+qed
 
 lemma mul_bin_union_eq_bin_union_mul: "X * (Y \<union> Z) = (X * Y) \<union> (X * Z)"
 proof-
-  have "X * (Y \<union> Z) = \<Union>{lift (X * y) X | y \<in> (Y \<union> Z)}" 
-    by (subst mul_eq_union_repl_lift_mul) auto
-  also have "... = \<Union>{lift (X * y) X | y \<in> Y} \<union> \<Union>{lift (X * y) X | y \<in> Z}"
-    by blast
-  also have "... = (X * Y) \<union> \<Union>{lift (X * y) X | y \<in> Z}"
-    by (subst mul_eq_union_repl_lift_mul) auto
-  also have "... = (X * Y) \<union> (X * Z)"
-    by (subst mul_eq_union_repl_lift_mul) auto
+  have "X * (Y \<union> Z) = \<Union>{lift (X * y) X | y \<in> (Y \<union> Z)}"
+    by (subst mul_eq_union_repl_lift_mul) simp
+  also have "... = \<Union>{lift (X * y) X | y \<in> Y} \<union> \<Union>{lift (X * y) X | y \<in> Z}" by blast
+  also have "... = (X * Y) \<union> (X * Z)" by (simp flip: mul_eq_union_repl_lift_mul)
   finally show ?thesis .
 qed
 
 lemma mul_union_eq_union_mul: "X * \<Union>Y = \<Union>(X * Y)"
 proof-
-  have "X * (\<Union>Y) = \<Union>{lift (X * y) X | y \<in> (\<Union>Y)}" 
+  have "X * (\<Union>Y) = \<Union>{lift (X * y) X | y \<in> (\<Union>Y)}"
     by (subst mul_eq_union_repl_lift_mul) auto
   also have "... = \<Union>\<Union>{lift (X * y) X | y \<in> Y}"
     sorry
@@ -516,7 +86,7 @@ proof-
 qed
 
 lemma unfolding_mul_union_eq_union_mul:
-"\<Union>{X * lift(Y * z) Y | z \<in> Z} = X * \<Union>{lift(Y * z) Y | z \<in> Z}"
+  "\<Union>{X * lift(Y * z) Y | z \<in> Z} = X * \<Union>{lift(Y * z) Y | z \<in> Z}"
   sorry
 
 lemma mul_lift_eq_lift_mul_mul: "X * (lift Y Z) = lift (X * Y) (X * Z)"
@@ -524,7 +94,7 @@ proof(induction Z rule:mem_induction)
   case (mem Z)
   have "X * (lift Y Z) = \<Union>{lift (X * z) X | z \<in> (lift Y Z)}"
     by (subst mul_eq_union_repl_lift_mul) auto
-  also have "... = \<Union>{lift (X * (Y + z)) X | z \<in> Z}" 
+  also have "... = \<Union>{lift (X * (Y + z)) X | z \<in> Z}"
     sorry
   also have "... = \<Union>{lift (X * Y + X * z) X | z \<in> Z}"
     sorry
@@ -547,7 +117,7 @@ proof(induction Z rule:mem_induction)
     by (auto simp: mem mul_lift_eq_lift_mul_mul)
   also have "... = X * \<Union>{lift(Y * z) Y | z \<in> Z}"
     by (auto simp: unfolding_mul_union_eq_union_mul)
-  also have "... = X * (Y * Z)" 
+  also have "... = X * (Y * Z)"
     by (subst mul_eq_union_repl_lift_mul) auto
   finally show ?case .
 qed
