HOTG/Axioms.thy
@@ -21,7 +21,7 @@ where
   mem_induction: "(\<forall>X. (\<forall>x. mem x X \<longrightarrow> P x) \<longrightarrow> P X) \<longrightarrow> (\<forall>X. P X)" and
   emptyset: "\<not>(\<exists>x. mem x emptyset)" and
   union: "\<forall>X x. mem x (union X) \<longleftrightarrow> (\<exists>Y. mem Y X \<and> mem x Y)" and
-  replacement: "\<forall>X y. mem y (repl X F) \<longleftrightarrow> (\<exists>x. mem x X \<and> y = F x)"
+  replacement: "\<forall>X y. mem y (repl X f) \<longleftrightarrow> (\<exists>x. mem x X \<and> y = f x)"
 
 text \<open>Note: axioms @{thm mem_induction} and @{thm replacement} are axiom schemas
 in first-order logic. Moreover, @{thm replacement} takes a meta-level function \<open>F\<close>.}\<close>
@@ -81,8 +81,8 @@ text \<open>Lastly, we want to axiomatise the existence of Grothendieck universe
 This can be done in different ways. We again follow the approach from
 \<^cite>\<open>"brown_et_al:LIPIcs:2019:11064"\<close>.\<close>
 
-definition mem_trans :: \<open>set \<Rightarrow> bool\<close>
-  where "mem_trans X \<equiv> (\<forall>x. x \<in> X \<longrightarrow> x \<subseteq> X)"
+definition mem_trans_closed :: \<open>set \<Rightarrow> bool\<close>
+  where "mem_trans_closed X \<equiv> (\<forall>x. x \<in> X \<longrightarrow> x \<subseteq> X)"
 
 definition ZF_closed :: \<open>set \<Rightarrow> bool\<close>
   where "ZF_closed U \<equiv> (
@@ -99,9 +99,9 @@ axiomatization
   univ :: \<open>set \<Rightarrow> set\<close>
 where
   mem_univ [iff]: "X \<in> univ X" and
-  mem_trans_univ [iff]: "mem_trans (univ X)" and
+  mem_trans_closed_univ [iff]: "mem_trans_closed (univ X)" and
   ZF_closed_univ [iff]: "ZF_closed (univ X)" and
-  univ_min: "\<lbrakk>X \<in> U; mem_trans U; ZF_closed U\<rbrakk> \<Longrightarrow> univ X \<subseteq> U"
+  univ_min: "\<lbrakk>X \<in> U; mem_trans_closed U; ZF_closed U\<rbrakk> \<Longrightarrow> univ X \<subseteq> U"
 
 (* Bundles to switch basic hotg notations on and off *)
 bundle hotg_basic_syntax
