HOTG/Arithmetics/Less_Than.thy
@@ -1,0 +1,33 @@
+theory Less_Than
+  imports
+    Transport.HOL_Syntax_Bundles_Orders
+    Foundation
+    Mem_Transitive_Closure
+begin
+
+unbundle no_HOL_ascii_syntax
+
+paragraph \<open>Less-Than Order\<close>
+
+definition "lt X Y \<equiv> X \<in> mem_trans_closure Y"
+
+bundle hotg_lt_syntax begin notation lt (infix "<" 60) end
+bundle no_hotg_lt_syntax begin no_notation lt (infix "<" 60) end
+unbundle hotg_lt_syntax
+unbundle no_HOL_order_syntax
+
+lemma lt_iff_mem_trans_closure: "X < Y \<longleftrightarrow> X \<in> mem_trans_closure Y"
+  unfolding lt_def by simp
+
+lemma lt_if_lt_if_mem [trans]:
+  assumes "y \<in> Y"
+  and "Y < X"
+  shows "y < X"
+  using assms mem_trans_closed_mem_trans_closure unfolding lt_iff_mem_trans_closure by auto
+
+lemma not_lt_self [iff]: "\<not>(X < X)"
+  using lt_iff_mem_trans_closure by auto
+
+
+
+end
