HOTG/Arithmetics/Mem_Transitive_Closure.thy
@@ -1,0 +1,106 @@
+theory Mem_Transitive_Closure
+  imports
+    Transport.Functions_Injective
+    Functions_Restrict
+    Foundation
+    Union_Intersection
+begin
+
+(*TODO Kevin: rename to binary_relation_restrict*)
+unbundle no_restrict_syntax
+unbundle no_HOL_ascii_syntax
+
+overloading
+  fun_restrict_set \<equiv> "fun_restrict :: (set \<Rightarrow> 'a) \<Rightarrow> set \<Rightarrow> set \<Rightarrow> 'a"
+begin
+  definition "fun_restrict_set f X \<equiv> f\<restriction>\<^bsub>mem_of X\<^esub> :: set \<Rightarrow> 'a"
+end
+
+lemma fun_restrict_set_eq_fun_restrict [simp]: "(f :: set \<Rightarrow> 'a)\<restriction>\<^bsub>X\<^esub> = f\<restriction>\<^bsub>mem_of X\<^esub>"
+  unfolding fun_restrict_set_def by auto
+
+axiomatization transrec :: "((set \<Rightarrow> 'a) \<Rightarrow> set \<Rightarrow> 'a) \<Rightarrow> set \<Rightarrow> 'a"
+  where transrec_eq: "transrec f X = f ((transrec f)\<restriction>\<^bsub>X\<^esub>) X"
+
+paragraph \<open>Transitive Closure\<close>
+
+definition "image f A \<equiv> {f x | x \<in> A}"
+
+lemma image_eq_repl [simp]: "image f A = repl A f"
+  unfolding image_def by simp
+
+lemma repl_fun_restrict_eq_repl [simp]: "{f\<restriction>\<^bsub>A\<^esub> x | x \<in> A} = {f x | x \<in> A}"
+  by simp
+
+lemma injective_image_if_injective:
+  assumes "injective f"
+  shows "injective (image f)"
+  by (intro injectiveI eqI) (use assms in \<open>auto dest: injectiveD\<close>)
+
+lemma injective_if_injective_image:
+  assumes "injective (image f)"
+  shows "injective f"
+proof (rule injectiveI)
+  fix X Y assume "f X = f Y"
+  then have "image f {X} = image f {Y}" by simp
+  with assms show "X = Y" by (blast dest: injectiveD)
+qed
+
+corollary injective_image_iff_injective [iff]: "injective (image f) \<longleftrightarrow> injective f"
+  using injective_image_if_injective injective_if_injective_image by blast
+
+
+definition "mem_trans_closure \<equiv> transrec (\<lambda>f X. X \<union> \<Union>(image f X))"
+
+lemma mem_trans_closure_eq_bin_union_repl:
+  "mem_trans_closure X = X \<union> \<Union>{mem_trans_closure x | x \<in> X}"
+  by (simp add: mem_trans_closure_def transrec_eq[where ?X=X])
+
+corollary subset_mem_trans_closure_self: "X \<subseteq> mem_trans_closure X"
+  by (auto simp: mem_trans_closure_eq_bin_union_repl[where ?X= X])
+
+corollary mem_mem_trans_closure_if_mem: "X \<in> Y \<Longrightarrow> X \<in> mem_trans_closure Y"
+  using subset_mem_trans_closure_self by blast
+
+corollary mem_mem_trans_closure_if_mem_union:
+  assumes "X \<in> \<Union>{mem_trans_closure x | x \<in> Y}"
+  shows "X \<in> mem_trans_closure Y"
+  using assms by (subst mem_trans_closure_eq_bin_union_repl) auto
+
+lemma mem_mem_trans_closureE [elim]:
+  assumes "X \<in> mem_trans_closure Y"
+  obtains (mem) "X \<in> Y" | (mem_trans_closure) y where "y \<in> Y" "X \<in> mem_trans_closure y"
+  using assms by (subst (asm) mem_trans_closure_eq_bin_union_repl) auto
+
+lemma mem_trans_closure_empty_eq_empty [simp]: "mem_trans_closure {} = {}"
+  by (simp add: mem_trans_closure_eq_bin_union_repl[where ?X="{}"])
+
+lemma mem_trans_closed_mem_trans_closure: "mem_trans_closed (mem_trans_closure X)"
+proof (induction X)
+  case (mem X)
+  show ?case
+  proof (rule mem_trans_closedI')
+    fix x y assume "x \<in> mem_trans_closure X" "y \<in> x"
+    then show "y \<in> mem_trans_closure X"
+    proof (cases rule: mem_mem_trans_closureE)
+      case mem
+      moreover have "y \<in> mem_trans_closure x" using \<open>y \<in> x\<close> subset_mem_trans_closure_self by blast
+      ultimately show ?thesis by (subst mem_trans_closure_eq_bin_union_repl) blast
+    next
+      case mem_trans_closure
+      with \<open>y \<in> x\<close> mem.IH show ?thesis by (subst mem_trans_closure_eq_bin_union_repl) blast
+    qed
+  qed
+qed
+
+lemma not_mem_trans_closure_self [iff]: "X \<notin> mem_trans_closure X"
+proof
+  assume "X \<in> mem_trans_closure X"
+  then show False
+  proof (cases rule: mem_mem_trans_closureE)
+    case (mem_trans_closure x)
+    with mem_trans_closed_mem_trans_closure show ?thesis by (induction X arbitrary: x) blast
+  qed auto
+qed
+
+end
