HOTG/Mem_Transitive_Closed.thy
@@ -1,0 +1,18 @@
+\<^marker>\<open>creator "Kevin Kappelmann"\<close>
+section \<open>Transitive Sets\<close>
+theory Mem_Transitive_Closed
+  imports Subset
+begin
+
+lemma mem_trans_closedI [intro]: "(\<And>x. x \<in> X \<Longrightarrow> x \<subseteq> X) \<Longrightarrow> mem_trans_closed X"
+  unfolding mem_trans_closed_def by auto
+
+lemma mem_trans_closedI': "(\<And>x y. x \<in> X \<Longrightarrow> y \<in> x \<Longrightarrow> y \<in> X) \<Longrightarrow> mem_trans_closed X"
+  by auto
+
+lemma mem_trans_closedD [dest]:
+  assumes "mem_trans_closed x"
+  shows "\<And>y. y \<in> x \<Longrightarrow> y \<subseteq> x"
+  using assms unfolding mem_trans_closed_def by auto
+
+end
